coq/ssrnat_ext.v
@@ -8,7 +8,11 @@ Ltac arith_hypo_ssrnat2coqnat :=
     | H : context [?L <= ?R] |- _ => move/leP: H => H
     | H : context [eqn ?L ?R] |- _ => move/eqnP: H => H
     | H : context [addn ?L ?R] |- _ => rewrite -plusE in H
+    | H : context [subn ?L ?R] |- _ => rewrite -subnE in H
     | H : context [muln ?L ?R] |- _ => rewrite -multE in H
+    | H : context [addn_rec ?L ?R] |- _ => rewrite /addn_rec in H
+    | H : context [subn_rec ?L ?R] |- _ => rewrite /subn_rec in H
+    | H : context [muln_rec ?L ?R] |- _ => rewrite /muln_rec in H
   end.
 
 Ltac arith_goal_ssrnat2coqnat :=
@@ -23,4 +27,4 @@ Ltac arith_goal_ssrnat2coqnat :=
 Ltac ssromega :=
   repeat arith_hypo_ssrnat2coqnat ;
   arith_goal_ssrnat2coqnat ;
-  omega.
+  (omega || apply False_ind; omega).
